%!TEX root = main.tex
% vim: tw=0 noet sts=8 sw=8

\section{The triple Massey product}

%first definition of the massey product for the n=3 case
\begin{DefLem}[Massey triple Product]
	Let $ (\Gamma,\d,\mu) $ a differential, graded
	algebra and let $ u\in\Gamma^p,v\in\Gamma^q,w\in\Gamma^r $ representatives of $ [u]\in H^p(\Gamma),[v]\in H^q(\Gamma) $
	and $ [w]\in H^r(\Gamma) $ such that $ [u][v] = [v][w] = 0 $.
	Then there exist $ s\in\Gamma^{p+q-1}, t\in\Gamma^{q+r-1} $ 
	such that $ \d s =\bar{u}v $ and $  \d t= \bar{v}w $. Then
	$ \bar{s}w + \bar{u}t$ is a cocycle and we can define the \textit{massey triple product} by
	\begin{align*}
	\massp{u}{v}{w} \coloneqq &\{ \;[\bar{s}w + \bar{u}t]\in H^{p+q+r-1}(\Gamma) \;\big|\; s\in H^{p+q-r},t\in H^{q+r-1} \\
	&\text{ such that } \d s = \bar{u}v,\d t = \bar{v}w \;\}.
	\end{align*} 
	\begin{proof}
		Let $ u,v,w,s,t $ as above and consider \todo{more exactly}
		\begin{align*}
		\d (\bar{s}w + \bar{u}t) &=  \d(\bar{s})w + (-1)^{1+\deg(\bar{s})} \underbrace{\d(w)}_{=0} + \underbrace{\d(\bar{u})}_{=0}t + (-1)^{\deg(\bar{u})} \bar{u} \d(t) \\
		&= (-1)^{1+\deg(\bar{s})} \d(s) w + (-1)^{\deg(\bar{u})} u\d(t)  \\
		&=  (-1)^{1+p+q-1} \bar{u}vw + (-1)^{1+p+q} \bar{u}vw = 0.\\
		\end{align*}
		Now the definition of the massey product is well-defined.
	\end{proof}
\end{DefLem}

\begin{Thm}
	Let $ \massp{u}{v}{w} $ a well-defined Massey triple product of
	the elements $ u\in\Gamma^p,v\in\Gamma^q$ and $ w\in\Gamma^r $,
	then it's a element of 
	\begin{gather*}
			 H^{p+q+r-1}(\Gamma) / \left([u]\cdot H^{q+r-1}(\Gamma) + H^{p+q-1}(\Gamma)\cdot [w] \right)
	\end{gather*}
	\begin{proof}
		\todo{show that different choices does not affect the massey product}
	\end{proof}
\end{Thm}


%%%% Local Variables:
%%%% mode: latex
%%%% TeX-master: "main"
%%%% End:
